Strata/DL/Imperative/StmtSemantics.lean
@@ -1208,7 +1208,7 @@ end -- section
 
 section
 
-variable (P : PureExpr) [HasFvar P] [HasBool P] [HasNot P]
+variable (P : PureExpr) [HasFvar P] [HasBool P] [HasNot P] [HasVarsPure P P.Expr]
 variable (extendEval : ExtendEval P)
 
 /-! ## Assertion Identity -/
@@ -1349,7 +1349,7 @@ theorem noMatchingAssert_implies_no_reachable_assert
   induction hstar_c with
   | refl => exact hno_c
   | step _ _ _ hstep _ ih =>
-    exact ih (@step_preserves_noMatchingAssert P _ _ _ extendEval _ _ _ hstep hno_c)
+    exact ih (@step_preserves_noMatchingAssert P _ _ _ _ extendEval _ _ _ hstep hno_c)
 
 /-! ## isAtAssert inversion lemmas -/
 
